![[functions.pdf]]
## 1
### 1a
$f(6) = (1/2)(6) + 4 = 3 + 4 = 7$

### 1b
$fg(-3) = f(g(-3)) = f((2(-3))/(x+1)) = f(-6 / -2) = f(3) = 0.5(3) + 4 = 5.5$

### 1c
$g(a) = -2; 2a/(a+1) = -2; 2a = -2a -2; a = -a -1, 2a = -1, a = -0.5$ 

### 1d
$y = 0.5x + 4; 0.5x = y - 4; x = 2(y - 4) = 2y-8$
$∴ f^–1(x) = 2x-8$

## 2
### 2a
#### 2ai
-2, because the denominator cannot be zero.

#### 2aii
Any value less than or equal to 1.

### 2b
$f(g(10)) = f(sqrt(10 -1)) = f(3) = 1/(3+2) = 0.2$

### 2c
$x^2 + 1$

## 3
### 3a
#### 3ai
$f(3) = 2(3)-1 = 5$

#### 3aii
$fg(6) = f(g(6)) = f(3/6) = f(0.5) = 1-1 = 0$

### 3b
$(x - 1)/2$

### 3c
#### 3ci
$gf(x) = 3/f(x) = 3/(2x-1)$

#### 3cii
The denominator cannot be zero, so: $2x-1 = 0, x = 0.5$

## 4
### 4a
$f(8) = (8-6)/2 = 2/2 = 1$

### 4b
$f^-1(x) = 2x + 6$

### 4c
The value of (x - 4) must be greater than zero, therefore, values of four and under cannot be included in the domain of g.

### 4d
$gf(x) = g(f(x)) = sqrt(((x-6)/2)-4) = sqrt((x-6-8)/2) = sqrt((x-14)/2)$

## 5
### 5a
#### 5ai
$f(3) = 3/(3-1) = 3/2 = 1.5$

#### 5aii 
$f(-3) = -3/(-3-1) = -3/-4 = 0.75$

### 5b
The denominator $(x - 1)$ cannot be zero, therefore, $(x-1) = 0; x = 1$

### 5c
$ff(x) = f(f(x)) = f(x/(x-1)) = (x/(x-1))/((x/(x-1)-1) = x$

## 6
### 6a
$f(11) = 2(11)/ (11-1) = 22 / 10 = 2.2$

### 6b
The denominator, $(x-1)$, cannot be zero, therefore, $x-1 = 0, x = 1$

### 6c
$y = 2x/(x-1)$, where $x = f^-1(y)$
*I can't figure out how to do this one*

### 6d
*I can't figure out how to do this one*

## 7

Tags: #math #surya #incomplete 
